Aoc24/Day16.lean
@@ -1,0 +1,132 @@
+import Aoc24.Utils
+import Aoc24.Direction
+import Aoc24.PriorityQueue
+
+-- https://www.dorais.org/lean4-parser/doc/
+
+-- input: 141×141
+
+open System Parser
+
+namespace Day16
+
+def testinput1 : FilePath := "input_16_test1"
+def testinput2 : FilePath := "input_16_test2"
+def realinput : FilePath := "input_16"
+
+/-
+PART 1:
+-/
+
+structure DijkstraData (n m : Nat) where
+  grid : Vector₂ Char n m
+  distances : Std.HashMap (Nat × Nat × NSEW) Nat
+  queue : PriorityQueue Nat (Nat × Nat × NSEW)
+
+def getGrid : StateM (DijkstraData n m) (Vector₂ Char n m) := do
+  let ⟨grid, _, _,⟩ ← get
+  return grid
+
+def wasVisited (y x : Nat) (dir : NSEW) : StateM (DijkstraData n m) Bool := do
+  let ⟨_, v, _,⟩ ← get
+  return v.contains ⟨y, x, dir⟩
+
+def visit (y x : Nat) (dir : NSEW) (dist : Nat) : StateM (DijkstraData n m) Unit := do
+  let ⟨g, v, q⟩ ← get
+  let v' := v.insert ⟨y, x, dir⟩ dist
+  set (σ := DijkstraData n m) ⟨g, v', q⟩
+
+def popQueue : StateM (DijkstraData n m) (Option (Nat × Nat × Nat × NSEW)) := do
+  let ⟨g, v, q⟩ ← get
+  match q with
+  | [] => return none
+  | head :: tail =>
+      set (σ := DijkstraData n m) ⟨g, v, tail⟩
+      return some head
+
+def requeue (prio y x : Nat) (dir : NSEW) : StateM (DijkstraData n m) Unit := do
+  let ⟨g, v, q⟩ ← get
+  let q' := q.insertOrLowerPriority prio ⟨y, x, dir⟩
+  set (σ := DijkstraData n m) ⟨g, v, q'⟩
+
+partial def dijkstra : StateM (DijkstraData n m) Unit := do
+  let some ⟨dist, y, x, dir⟩ ← popQueue | return
+  visit y x dir dist
+  let grid ← getGrid
+  let ⟨ny, nx⟩ := dir.step y x 1
+  if grid[ny]![nx]! != '#' && !(← wasVisited ny nx dir) then
+    requeue (dist + 1) ny nx dir
+  for ndir in [dir.rotateCCW, dir.rotateCW] do
+    if !(← wasVisited y x ndir) then
+      requeue (dist + 1000) y x ndir
+  dijkstra
+
+def getMin (l : List (Option Nat)) : Option Nat :=
+  l.foldl (init := none) fun cur new =>
+    match cur, new with
+    | none, _ => new
+    | some x, none => some x
+    | some x, some y => if x ≤ y then some x else some y
+
+def getDist (distances : Std.HashMap (Nat × Nat × NSEW) Nat) (y x : Nat) : Option (Nat × NSEW) :=
+  let dn := distances[(⟨y, x, .n⟩ : Nat × Nat × NSEW)]?
+  let ds := distances[(⟨y, x, .s⟩ : Nat × Nat × NSEW)]?
+  let de := distances[(⟨y, x, .e⟩ : Nat × Nat × NSEW)]?
+  let dw := distances[(⟨y, x, .w⟩ : Nat × Nat × NSEW)]?
+  let m := getMin [dn, ds, de, dw]
+  match m with
+  | none => none
+  | some d =>
+      if m == dn then some ⟨d, .n⟩
+      else if m == ds then some ⟨d, .s⟩
+      else if m == de then some ⟨d, .e⟩
+      else some ⟨d, .w⟩
+
+
+def firstPart (input : FilePath) : IO Nat := do
+  let raw := (← IO.FS.lines input)
+  let some ⟨n, m, grid⟩ := raw.map (·.toCharArray) |>.toVector₂ | IO.exitWithError "parse error";
+  let some ⟨sy, sx⟩ := grid.findElem 'S' | IO.exitWithError "Can't find start"
+  let some ⟨ey, ex⟩ := grid.findElem 'E' | IO.exitWithError "Can't find end"
+  let initdata : DijkstraData n m := ⟨grid, .empty, [⟨0, sy, sx, .e⟩]⟩
+  let ⟨_, distances, _⟩ := dijkstra.runState initdata
+  let some ⟨d, _⟩ := getDist distances ey ex | IO.exitWithError "did not reach E"
+  return d
+
+--#eval firstPart testinput1           --(ans: 7036)
+--#eval firstPart testinput2           --(ans: 11048)
+--#eval firstPart realinput           --(ans: )
+
+/-
+PART 2:
+-/
+
+def secondPart (input : FilePath) : IO Nat := do
+  let raw := (← IO.FS.lines input)
+  let some ⟨n, m, grid⟩ := raw.map (·.toCharArray) |>.toVector₂ | IO.exitWithError "parse error";
+  let some ⟨sy, sx⟩ := grid.findElem 'S' | IO.exitWithError "Can't find start"
+  let some ⟨ey, ex⟩ := grid.findElem 'E' | IO.exitWithError "Can't find end"
+  let initdata₁ : DijkstraData n m := ⟨grid, .empty, [⟨0, sy, sx, .e⟩]⟩
+  let ⟨_, distancesFromS, _⟩ := dijkstra.runState initdata₁
+  let some ⟨d, dir⟩ := getDist distancesFromS ey ex | IO.exitWithError "did not reach E"
+  let initdata₂ : DijkstraData n m := ⟨grid, .empty, [⟨0, ey, ex, dir.reverse⟩]⟩
+  let ⟨_, distancesFromE, _⟩ := dijkstra.runState initdata₂
+  let mut out := 0
+  for y in [:n] do
+    for x in [:m] do
+      let mut flag := false
+      for dir in [NSEW.n, .s, .e, .w] do
+        match distancesFromS[(⟨y, x, dir⟩ : Nat × Nat × NSEW)]? with
+        | none => noop
+        | some dist₁ =>
+          match distancesFromE[(⟨y, x, dir.reverse⟩ : Nat × Nat × NSEW)]? with
+          | none => noop
+          | some dist₂ => if dist₁ + dist₂ == d then flag := true
+      if flag then out := out + 1
+  return out
+
+--#eval secondPart testinput1           --(ans: )
+--#eval secondPart testinput2           --(ans: )
+--#eval secondPart realinput           --(ans: )
+
+end Day16
