Aoc24/PriorityQueue.lean
@@ -1,0 +1,46 @@
+/- I should use the following, but changing priorities is not
+implemented yet -/
+
+--abbrev PriorityQueue (α : Type _) [Ord α] (β : Type _) :=
+--  Batteries.BinomialHeap (α × β) (fun x y => compare x.1 y.1 != .gt)
+
+abbrev PriorityQueue (α : Type _) [Ord α] (β : Type _) := List (α × β)
+
+namespace PriorityQueue
+
+variable [Ord α]
+
+def empty : PriorityQueue α β := []
+
+def insert [BEq β] (q : PriorityQueue α β) (p : α) (x : β) : PriorityQueue α β :=
+  match q with
+  | [] => [⟨p, x⟩]
+  | ⟨p', x'⟩ :: tail =>
+      match compare p p' with
+      | .gt => ⟨p', x'⟩ :: PriorityQueue.insert tail p x
+      | _ => if x != x' then ⟨p, x⟩ :: ⟨p', x'⟩ :: tail else ⟨p, x⟩ :: tail
+
+def extractMin (q : PriorityQueue α β) : Option (α × β) := q.head?
+
+-- Only acts on the first one it finds
+def deleteElem [BEq β] (q : PriorityQueue α β) (x : β) : PriorityQueue α β :=
+  match q with
+  | [] => []
+  | ⟨p', x'⟩ :: tail =>
+      if x != x' then ⟨p', x'⟩ :: deleteElem tail x
+      else tail
+
+def deleteElemIfAbove [BEq β] (q : PriorityQueue α β) (prio : α) (x : β) : PriorityQueue α β :=
+  match q with
+  | [] => []
+  | ⟨p', x'⟩ :: tail =>
+      if x != x' then ⟨p', x'⟩ :: deleteElemIfAbove tail prio x
+      else
+        if compare prio p' == .lt then tail else q
+
+def insertOrLowerPriority [BEq β] (q : PriorityQueue α β) (p : α) (x : β) :
+    PriorityQueue α β :=
+  let q' := q.deleteElemIfAbove p x
+  q'.insert p x
+
+end PriorityQueue
